Extracted step function
* step is now a common function that consider the first element of the
  "frontier" (stack, queue, prio-queue) and calls expand on it.
* only the expand function still differs from search to search

Graphlib/BFS.lean
@@ -6,159 +6,42 @@ import Mathlib.Data.List.MinMax
 import Graphlib.Lists
 import Graphlib.FinEnum
 import Graphlib.Basic
+import Graphlib.SearchState
+import Graphlib.SearchAlgorithm
+import Graphlib.SearchStep
 
 set_option trace.split.failure true
 --set_option diagnostics true
 
 -- def local global variable for a graph
 variable {V : Type} {E : Type} [FinEnum V] [DecidableEq V] [DecidableEq E]
-variable (G : WeightedDiGraph V E)
-
-
+variable {g : WeightedDiGraph V E}
 
 -----------------------------------------------------------------------
------- Search state of the bfs and its invariants
-structure bfs_state [FinEnum V] [DecidableEq E] [DecidableEq V]
-    (g: WeightedDiGraph V E) (start : V) where
-    visited : Finset V
-    pathOrder : V → Nat 
-    mother : visited → V
-    mother_proof (v : visited): ↑v ≠ start → g.Adj (mother v) v
-    stack : List V
-    terminated : Bool
-
-abbrev bfs_invar_stack_is_visited [FinEnum V] [DecidableEq E] [DecidableEq V]
-    (g: WeightedDiGraph V E) (start : V) (s : bfs_state g start):=
-      ∀ x : V, x ∈ s.stack → x ∈ s.visited
-
-abbrev bfs_invar_mother_is_visited [FinEnum V] [DecidableEq E] [DecidableEq V]
-    (g: WeightedDiGraph V E) (start : V) (s : bfs_state g start):=
-      ∀ x : s.visited, s.mother x ∈ s.visited
-
-abbrev bfs_invar_mother_decreasing_path_order [FinEnum V] [DecidableEq E] [DecidableEq V]
-    (g: WeightedDiGraph V E) (start : V) (s : bfs_state g start) :=
-      ∀ x : s.visited, ↑x ≠ start → s.pathOrder (s.mother x) < s.pathOrder x 
-
-abbrev bfs_invar_on_stack_or_all_neighbours_visited [FinEnum V] [DecidableEq E] [DecidableEq V]
-    (g: WeightedDiGraph V E) (start : V) (s : bfs_state g start):=
-      ∀ x : s.visited, ↑x ∈ s.stack ∨ ∀ y : V, (g.Adj x y) → y ∈ s.visited
-
-abbrev bfs_invar_start_visited [FinEnum V] [DecidableEq E] [DecidableEq V]
-    (g: WeightedDiGraph V E) (start : V) (s : bfs_state g start) :=
-      start ∈ s.visited
-
-def extract_path_to [FinEnum V] [DecidableEq E] [DecidableEq V]
-    (g: WeightedDiGraph V E) (start : V) (goal : V) (search_state : bfs_state g start)
-    (goal_reached : goal ∈ search_state.visited)
-    (mother_invar : bfs_invar_mother_is_visited g start search_state)
-    (decreasing_invar : bfs_invar_mother_decreasing_path_order g start search_state):
-      Σ' (p : Path g start goal), (∀ v ∈ support g p.walk, search_state.pathOrder v ≤ search_state.pathOrder goal):= 
-      if start_is_goal : goal = start then
-        let emptyW : Walk g start goal := start_is_goal ▸ Walk.nil
-        let emptyP : Path g start goal := Path.mk emptyW (by
-          simp [emptyW]
-          unfold support
-          split
-          · next u u' x w rest u_adj_v walk_is_cons => 
-            simp_all
-            subst start_is_goal
-            simp_all only [reduceCtorEq] 
-          · simp
-        )
-
-        have order : ∀ v ∈ support g emptyP.walk, search_state.pathOrder v ≤ search_state.pathOrder goal := by
-          intro a a_in_support
-          unfold emptyP at a_in_support
-          unfold emptyW at a_in_support
-          unfold support at a_in_support
-          simp_all
-          subst start_is_goal
-          simp_all only [List.mem_cons, List.not_mem_nil, or_false, le_refl]
-
-        ⟨ emptyP, order ⟩ 
-      else
-        let goal_predecessor : V := search_state.mother ⟨ goal, goal_reached ⟩
-        let ⟨ path_start_pre, order_proof ⟩ := -- : Path g start goal_predecessor :=
-          extract_path_to g start goal_predecessor search_state (by apply mother_invar) mother_invar decreasing_invar 
-        let pre_adj_goal : g.Adj goal_predecessor goal := search_state.mother_proof ⟨ goal , goal_reached ⟩ start_is_goal
-        let goal_not_visited : goal ∉ support g path_start_pre.walk := by
-          by_contra goal_is_in_support
-          have h := order_proof goal goal_is_in_support
-          unfold goal_predecessor at h
-          unfold bfs_invar_mother_decreasing_path_order at decreasing_invar
-          have h' := decreasing_invar ⟨ goal, goal_reached⟩ 
-          clear mother_invar decreasing_invar
-          simp_all
-          omega
-
-        let goal_path : Path g start goal := extend_path g path_start_pre pre_adj_goal goal_not_visited
-
-        let new_order_proof : ∀ v ∈ support g goal_path.walk, search_state.pathOrder v ≤ search_state.pathOrder goal := by
-          intro a a_in_support
-          unfold goal_path at a_in_support
-          rw [extend_path_extends_support] at a_in_support
-          simp_all
-          apply a_in_support.elim
-          · intro a_in_old_path
-            apply le_trans 
-            · apply order_proof
-              exact a_in_old_path
-            · unfold goal_predecessor
-              apply le_of_lt
-              exact decreasing_invar ⟨ goal,goal_reached ⟩ start_is_goal
-          · simp_all
-
-        ⟨ goal_path, new_order_proof ⟩ 
-
-termination_by search_state.pathOrder goal
-decreasing_by
-  simp_all only [Subtype.forall, ne_eq, not_false_eq_true]
-
-
------------------------------------------------------------------------
------- bfs implementation and proof ------
+------ BFS implementation and proof ------
 
 def bfs_step_expand[FinEnum V] [DecidableEq E] [DecidableEq V]
     (g: WeightedDiGraph V E)
-    (start : V)
-    (priorState : bfs_state g start)
+    (priorState : base_search_state g)
     (stackHead : V)
     (stackTail : List V):
-    (bfs_state g start) :=
+    (base_search_state g) :=
       let newly_visited : Finset V := (Finset.univ).filterMap
         (λ v => if @decide (g.Adj stackHead v) (g.instDecAdj stackHead v) ∧ v ∉ priorState.visited
                   then some v
                   else none)
         (by intro a a' b a_1 a_2; simp_all) -- filter neighbors to expand the visited list
-
       
       let vList : List V := (FinEnum.toList (Finset.univ : Finset V))
       let newly_visited_list : List V :=
         vList.filterMap (λ v => if v ∈ newly_visited then some v else none)
       let new_visited : Finset V := priorState.visited ∪ newly_visited
-      let new_stack : List V := stackTail ++ newly_visited_list  -- add neighbors in front to stack
+      let new_stack : List V := stackTail ++ newly_visited_list -- add neighbors at end of stack
      
       let new_mother : new_visited → V := fun ⟨v, hv⟩  =>
         if h: (v ∈ priorState.visited) then priorState.mother ⟨ v, by exact h⟩
         else stackHead
       
-      let new_mother_proof (v : new_visited): ↑v ≠ start → g.Adj (new_mother v) v :=
-       fun not_start =>
-        by
-          unfold new_mother
-          simp_all
-          split
-          · next prior_visited_v =>
-            exact priorState.mother_proof ⟨↑v, prior_visited_v⟩ not_start
-          · next not_prior_visited_v => 
-            obtain ⟨ vv, v_new_visited ⟩ := v
-            unfold new_visited at v_new_visited
-            simp_all
-            simp at v_new_visited
-            simp_all
-            unfold newly_visited at v_new_visited
-            simp_all
-
       let new_order : V → Nat := fun v  =>
         if h: (v ∈ priorState.visited) then priorState.pathOrder v
         else if hh : (priorState.visited.card = 0) then 0
@@ -166,37 +49,31 @@ def bfs_step_expand[FinEnum V] [DecidableEq E] [DecidableEq V]
         else 1 + priorState.pathOrder stackHead
         -- priorState.stack.length
       
-      bfs_state.mk new_visited new_order new_mother new_mother_proof new_stack false
+      base_search_state.mk new_visited new_order new_mother new_stack
 
 
-lemma bfs_expand_newly_added_are_adjacent --[FinEnum V] [DecidableEq E] [DecidableEq V]
-    (g: WeightedDiGraph V E)
-    (start : V)
-    (priorState : bfs_state g start)
+lemma bfs_expand_newly_added_are_adjacent 
+    (priorState : base_search_state g)
     (stackHead : V)
     (stackTail : List V):
     ∀ x : V, x ∉ priorState.visited ∧ x ∉ stackTail ∧
-      x ∈ (bfs_step_expand g start priorState stackHead stackTail).stack →  
+      x ∈ (bfs_step_expand g priorState stackHead stackTail).stack →  
       g.Adj stackHead x := by
-    intro x
-    intro ⟨x_not_visi, ⟨ x_not_on_stack_before, x_on_stack_after ⟩  ⟩
+    intro x ⟨x_not_visi, ⟨ x_not_on_stack_before, x_on_stack_after ⟩  ⟩
     unfold bfs_step_expand at x_on_stack_after
     simp_all
 
 
-lemma bfs_expand_keeps_stack_in_visited --[FinEnum V] [DecidableEq E] [DecidableEq V]
-    (g: WeightedDiGraph V E)
-    (start : V)
-    (priorState : bfs_state g start)
+lemma bfs_expand_keeps_stack_in_visited 
+    (priorState : base_search_state g)
     (stackHead : V)
     (stackTail : List V):
-    bfs_invar_stack_is_visited g start priorState ∧
+    search_invar_stack_is_visited priorState ∧
       stackHead ∈ priorState.visited ∧ (∀ x : V, x ∉ priorState.visited → x ∉ stackTail) →
-      bfs_invar_stack_is_visited g start (bfs_step_expand g start priorState stackHead stackTail) := by
+      search_invar_stack_is_visited (bfs_step_expand g priorState stackHead stackTail) := by
       intro ⟨ stack_is_visited_prior, stackhead_visited, x_not_in_stack_tail⟩ 
-      unfold bfs_invar_stack_is_visited
-      intro x 
-      intro x_now_on_stack
+      unfold search_invar_stack_is_visited
+      intro x x_now_on_stack
       unfold bfs_step_expand
       simp_all
       by_cases x_was_visited : x ∈ priorState.visited
@@ -204,20 +81,18 @@ lemma bfs_expand_keeps_stack_in_visited --[FinEnum V] [DecidableEq E] [Decidable
         exact x_was_visited
       · right
         apply And.intro
-        · apply (bfs_expand_newly_added_are_adjacent g start priorState stackHead stackTail)
+        · apply (bfs_expand_newly_added_are_adjacent priorState stackHead stackTail)
           simp_all
         · exact x_was_visited
 
 
-lemma bfs_expand_keeps_mother_in_visited --[FinEnum V] [DecidableEq E] [DecidableEq V]
-    (g: WeightedDiGraph V E)
-    (start : V)
-    (priorState : bfs_state g start)
+lemma bfs_expand_keeps_mother_in_visited 
+    (priorState : base_search_state g)
     (stackHead : V)
     (stackTail : List V):
-    bfs_invar_mother_is_visited g start priorState ∧ stackHead ∈ priorState.visited → bfs_invar_mother_is_visited g start (bfs_step_expand g start priorState stackHead stackTail) := by
+    search_invar_mother_is_visited priorState ∧ stackHead ∈ priorState.visited → search_invar_mother_is_visited (bfs_step_expand g priorState stackHead stackTail) := by
       intro mother_is_visited_prior
-      unfold bfs_invar_mother_is_visited
+      unfold search_invar_mother_is_visited
       intro x
       simp_all
       unfold bfs_step_expand
@@ -226,22 +101,40 @@ lemma bfs_expand_keeps_mother_in_visited --[FinEnum V] [DecidableEq E] [Decidabl
       all_goals
         simp_all
 
-
-
-lemma bfs_expand_keeps_mother_ordered --[FinEnum V] [DecidableEq E] [DecidableEq V]
-    (g: WeightedDiGraph V E)
+lemma bfs_expand_keeps_mother_is_adjacent
     (start : V)
-    (priorState : bfs_state g start)
+    (priorState : base_search_state g)
     (stackHead : V)
     (stackTail : List V):
-    bfs_invar_mother_is_visited g start priorState ∧
+    search_invar_mother_is_adjacent start priorState → search_invar_mother_is_adjacent start (bfs_step_expand g priorState stackHead stackTail) := by
+      intro mother_is_adjacent_prior
+      unfold search_invar_mother_is_adjacent
+      intro x
+      simp_all
+      intro x_not_start
+      unfold bfs_step_expand
+      simp_all
+      split
+      · simp_all
+      · next x_not_prior_visited => 
+        obtain ⟨ xx, x_in_new_visited ⟩ := x
+        unfold bfs_step_expand at x_in_new_visited
+        simp at x_in_new_visited
+        simp_all
+
+lemma bfs_expand_keeps_mother_ordered 
+    (start : V)
+    (priorState : base_search_state g)
+    (stackHead : V)
+    (stackTail : List V):
+    search_invar_mother_is_visited priorState ∧
       stackHead ∈ priorState.visited ∧ 
-      bfs_invar_mother_decreasing_path_order g start priorState
-      → bfs_invar_mother_decreasing_path_order g start
-          (bfs_step_expand g start priorState stackHead stackTail)
+      search_invar_mother_decreasing_path_order start priorState
+      → search_invar_mother_decreasing_path_order start
+          (bfs_step_expand g priorState stackHead stackTail)
           := by
     intro ⟨mother_is_visited, stack_head_visited_prior,mother_decreasing_prior⟩  
-    unfold bfs_invar_mother_decreasing_path_order
+    unfold search_invar_mother_decreasing_path_order
     intro a a_not_stat
     unfold bfs_step_expand
     simp_all
@@ -254,22 +147,18 @@ lemma bfs_expand_keeps_mother_ordered --[FinEnum V] [DecidableEq E] [DecidableEq
       · rw [Nat.add_comm]
         apply Nat.lt_succ_of_le
         apply le_refl
-        --apply maximum_path_order_is_le
-        --simp_all
 
 lemma bfs_expand_keeps_on_stack_or_all_neighbours_visited
-    (g: WeightedDiGraph V E)
-    (start : V)
-    (priorState : bfs_state g start)
+    (priorState : base_search_state g)
     (stackHead : V)
     (stackTail : List V):
-     bfs_invar_on_stack_or_all_neighbours_visited g start priorState
+     search_invar_on_stack_or_all_neighbours_visited priorState
      ∧ priorState.stack = (stackHead :: stackTail)
-     → bfs_invar_on_stack_or_all_neighbours_visited g start
-          (bfs_step_expand g start priorState stackHead stackTail)
+     → search_invar_on_stack_or_all_neighbours_visited  
+          (bfs_step_expand g priorState stackHead stackTail)
           := by
       intro ⟨ invar_holds_on_prior_state, stack_composition ⟩ 
-      unfold bfs_invar_on_stack_or_all_neighbours_visited
+      unfold search_invar_on_stack_or_all_neighbours_visited
       intro ⟨ x, x_now_on_stack⟩
       by_cases x_not_stack_head : x ≠ stackHead
       · by_cases x_was_not_in_stack_tail_: x ∈ stackTail
@@ -300,867 +189,190 @@ lemma bfs_expand_keeps_on_stack_or_all_neighbours_visited
         · right; exact h
 
 lemma bfs_expand_keeps_start_visited
-    (g: WeightedDiGraph V E)
     (start : V)
-    (priorState : bfs_state g start)
+    (priorState : base_search_state g)
     (stackHead : V)
     (stackTail : List V):
-     bfs_invar_start_visited g start priorState →
-     bfs_invar_start_visited g start (bfs_step_expand g start priorState stackHead stackTail)
+     search_invar_start_visited start priorState →
+     search_invar_start_visited start (bfs_step_expand g priorState stackHead stackTail)
           := by
       intro pre_invar
       unfold bfs_step_expand
-      unfold bfs_invar_start_visited 
+      unfold search_invar_start_visited 
       simp_all
 
----------------------------------------------------------------------------------------
--- run one step of the bfs. Mostly case distinction and running expansion if necessary
-def bfs_step [FinEnum V] [DecidableEq E] [DecidableEq V]
-    (g: WeightedDiGraph V E) (start : V) (goal : V)
-    (priorState : bfs_state g start) :
-    (bfs_state g start) × (Option Bool) :=
-  match priorState.stack with
-    | [] => ({priorState with terminated := true} , some false) -- goal not found
-    | (s :: xs) =>
-    if s = goal then ({priorState with terminated := true}, some true)
-    else
-      (bfs_step_expand g start priorState s xs, none)
-
-
-lemma bfs_step_visited_subset 
-    (g: WeightedDiGraph V E) (start : V) (goal : V)
-    (priorState : bfs_state g start) :
-    priorState.visited ⊆ (bfs_step g start goal priorState).1.visited := by
-    unfold bfs_step
-    split
-    · simp_all
-    split
-    · simp_all
+lemma bfs_expand_visited_subset (priorState : base_search_state g)
+    (stackHead : V)
+    (stackTail : List V):
+    priorState.visited ⊆ (bfs_step_expand g priorState stackHead stackTail).visited := by
     unfold bfs_step_expand
     simp_all
 
-lemma bfs_step_visited_is_smaller_than_V 
-    (g: WeightedDiGraph V E) (start : V) (goal : V)
-    (priorState : bfs_state g start):
-   (bfs_step g start goal priorState).1.visited.card ≤ Fintype.card V := by
-    apply Finset.card_le_univ
-  
-lemma bfs_step_visited_increases
-    (g: WeightedDiGraph V E) (start : V) (goal : V)
-    (priorState : bfs_state g start):
-      (bfs_step g start goal priorState).1.visited.card ≥ priorState.visited.card := by
-    change priorState.visited.card ≤ (bfs_step g start goal priorState).1.visited.card
-    apply Finset.card_le_card
-    apply bfs_step_visited_subset
-
-----------
--- the step also keeps the invariants
-lemma bfs_step_keeps_stack_in_visited 
-    (g: WeightedDiGraph V E)
-    (start : V)
-    (priorState : bfs_state g start):
-    ∀ goal : V,
-    bfs_invar_stack_is_visited g start priorState →
-      bfs_invar_stack_is_visited g start (bfs_step g start goal priorState).fst := by
-        intro goal
-        intro stack_is_visited_prior 
-        unfold bfs_step
-        split
-        · unfold bfs_invar_stack_is_visited
-          simp_all
-        next _ head tail head_tail_compose =>
-        split
-        · unfold bfs_invar_stack_is_visited
-          simp_all
-        apply bfs_expand_keeps_stack_in_visited
-        simp_all
-        constructor
-        · exact stack_is_visited_prior
-        intro y y_not_visited
-        intro y_in_tail
-        simp_all
-      
-
-
-lemma bfs_step_keeps_mother_in_visited 
-    (g: WeightedDiGraph V E)
-    (start : V)
-    (priorState : bfs_state g start):
-    ∀ goal : V,
-    bfs_invar_stack_is_visited g start priorState ∧ bfs_invar_mother_is_visited g start priorState →
-      bfs_invar_mother_is_visited g start (bfs_step g start goal priorState).fst := by
-      intro goal
-      intro ⟨ mother_is_visited_prior, stack_is_visited_prior ⟩ 
-      unfold bfs_step
-      split
-      · simp_all
-      next _ head tail head_tail_compose =>
-      split
-      · simp_all
-      apply bfs_expand_keeps_mother_in_visited
+lemma bfs_expand_keeps_goal_on_stack :
+    base_invar_carries_over_expand (state_type := base_search_state g) goal (bfs_step_expand g) (search_prop_goal_on_stack (g:=g) goal):= by
+    unfold base_invar_carries_over_expand
+    intro s head tail ⟨ goal_prior_on_stack, head_not_goal, compose⟩ 
+    change search_prop_goal_on_stack goal (bfs_step_expand g s head tail)
+    unfold bfs_step_expand
+    unfold search_prop_goal_on_stack at ⊢ goal_prior_on_stack
+    simp_all 
+    cases  goal_prior_on_stack
+    all_goals
       simp_all
 
-
-lemma bfs_step_keeps_mother_ordered
-    (g: WeightedDiGraph V E)
-    (start : V)(priorState : bfs_state g start):
-    ∀ goal : V,
-      bfs_invar_stack_is_visited g start priorState ∧
-      bfs_invar_mother_is_visited g start priorState ∧
-      bfs_invar_mother_decreasing_path_order g start priorState
-      → bfs_invar_mother_decreasing_path_order g start (bfs_step g start goal priorState).fst := by
-        intro goal
-        intro ⟨ stack_visited, mother_visited, mother_decreasing⟩ 
-        unfold bfs_step
-        split
-        · simp_all
-        next _ head tail head_tail_compose => 
-        split
-        · simp_all
-        apply bfs_expand_keeps_mother_ordered
-        simp_all
+lemma bfs_expand_goal_becomes_visited_puts_it_on_stack
+  (goal : V)
+  : 
+  goal_becomes_visited_puts_it_on_stack (g:=g) goal (bfs_step_expand g):= by
+    unfold goal_becomes_visited_puts_it_on_stack
+    intro s head tail ⟨ a,b,c,d⟩ 
+    change search_prop_goal_on_stack goal (bfs_step_expand g s head tail)
+    have bb : goal ∈ (bfs_step_expand g s head tail).visited := b
+    clear b
+    unfold bfs_step_expand at bb ⊢
+    unfold search_prop_goal_on_stack
+    simp_all
+    cases bb
+    · contradiction
+    · next h => left; exact h
 
 
-lemma bfs_step_keeps_on_stack_or_all_neighbours_visited
-    (g: WeightedDiGraph V E)
-    (start : V)(priorState : bfs_state g start):
-    ∀ goal : V,
-     bfs_invar_on_stack_or_all_neighbours_visited g start priorState
-     → bfs_invar_on_stack_or_all_neighbours_visited g start 
-          (bfs_step g start goal priorState).fst := by
-        intro goal
-        intro stack_or_neighbour_visited
-        unfold bfs_step
-        split
-        · simp_all
-          exact stack_or_neighbour_visited
-        next _ head tail head_tail_compose => 
-        split
-        · simp_all
-        apply bfs_expand_keeps_on_stack_or_all_neighbours_visited
-        simp_all
+lemma visited_is_smaller_than_V (state : base_search_state g): state.visited.card ≤ Fintype.card V := by
+    apply Finset.card_le_univ
+  
 
-lemma bfs_step_keeps_start_in_visited 
-    (g: WeightedDiGraph V E)
-    (start : V)
-    (priorState : bfs_state g start):
-    ∀ goal : V,
-    bfs_invar_start_visited g start priorState →
-      bfs_invar_start_visited g start (bfs_step g start goal priorState).fst := by
-        intro goal
-        intro stack_is_visited_prior 
-        unfold bfs_step
-        split
-        · unfold bfs_invar_start_visited
+lemma bfs_expand_visited_increases
+    (priorState : base_search_state g)
+    (head : V)
+    (tail : List V):
+      (bfs_step_expand g priorState head tail).visited.card ≥ priorState.visited.card := by
+    change priorState.visited.card ≤ (bfs_step_expand g priorState head tail).visited.card
+    apply Finset.card_le_card
+    apply bfs_expand_visited_subset
+
+
+lemma bfs_expand_keeps_base_invars:
+  base_invar_carries_over_expand goal (bfs_step_expand g) (search_invar_all_basic (g:=g) start) := by
+  unfold base_invar_carries_over_expand
+  unfold search_invar_all_basic
+  intro s head tail ⟨ ⟨ i1,i2,i3,i4,i5,i6⟩ , head_not_goal, compose⟩ 
+  have head_is_visited : head ∈ s.visited := by
+    apply i1
+    rw [compose]
+    simp
+  repeat rw [← and_assoc]
+  repeat constructor
+  · apply bfs_expand_keeps_stack_in_visited
+    constructor
+    · exact i1
+    · constructor
+      · exact head_is_visited 
+      · intro x x_not_visited
+        by_contra x_in_tail
+        have x_on_stack : x ∈ (has_base_search_state.to_base_state (g:=g) s).stack := by
+          rw [compose]
           simp_all
-        next _ head tail head_tail_compose =>
-        split
-        · unfold bfs_invar_start_visited
-          simp_all
-        apply bfs_expand_keeps_start_visited
-        simp_all
-
+        apply i1 at x_on_stack
+        contradiction 
+  · apply bfs_expand_keeps_mother_in_visited
+    constructor
+    · exact i2
+    · exact head_is_visited
+  · apply bfs_expand_keeps_mother_is_adjacent
+    exact i3
+  · apply bfs_expand_keeps_mother_ordered
+    constructor
+    · exact i2
+    · constructor
+      · exact head_is_visited
+      · exact i4
+  · apply bfs_expand_keeps_on_stack_or_all_neighbours_visited
+    constructor
+    · exact i5 
+    · exact compose 
+  · apply bfs_expand_keeps_start_visited
+    exact i6
 
 --------------------------------------------------------------------------------------------------
 -- main recursion loop 
 
-
-lemma termination_bfs_recurse 
-    (g: WeightedDiGraph V E) (start : V)(goal : V)
-    (priorState : bfs_state g start)
-    (nextState : bfs_state g start):
-    (nextState = (bfs_step g start goal priorState).1) ∧ (nextState.terminated = false)
+lemma termination_bfs_recurse
+    (priorState : base_search_state g)
+    (nextState : base_search_state g)
+    (head : V)
+    (tail : List V)
+    (compose : priorState.stack = head :: tail):
+    (nextState = (bfs_step_expand g priorState head tail))
     → ((Fintype.card V - nextState.visited.card < Fintype.card V - priorState.visited.card
         ∨ (Fintype.card V - nextState.visited.card = Fintype.card V - priorState.visited.card ∧ nextState.stack.length < priorState.stack.length)) ):= by
-  intro ⟨ nextStateDef, still_not_terminated ⟩
+  intro nextStateDef
   apply (Classical.or_iff_not_imp_left).mpr
   intro visited_not_decreasing
   simp_all
-  have same_visited : (bfs_step g start goal priorState).1.visited.card = priorState.visited.card := by
-    have k2 : (bfs_step g start goal priorState).1.visited.card ≤ Fintype.card V :=
-      bfs_step_visited_is_smaller_than_V g start goal priorState
-    have k3 : (bfs_step g start goal priorState).1.visited.card ≥ priorState.visited.card := 
-      bfs_step_visited_increases g start goal priorState
+  have same_visited : (bfs_step_expand g priorState head tail).visited.card = priorState.visited.card := by
+    have k2 : (bfs_step_expand g priorState head tail).visited.card ≤ Fintype.card V := by
+      apply visited_is_smaller_than_V 
+    have k3 : (bfs_step_expand g priorState head tail).visited.card ≥ priorState.visited.card := by
+      apply bfs_expand_visited_increases 
     omega
-  have visited_eq : priorState.visited = (bfs_step g start goal priorState).1.visited := by
+  have visited_eq : priorState.visited = (bfs_step_expand g priorState head tail).visited := by
     ext a
     constructor
     · apply Finset.mem_of_subset
-      apply bfs_step_visited_subset 
+      apply bfs_expand_visited_subset 
     apply finsetLemma
-    · apply bfs_step_visited_subset 
+    · apply bfs_expand_visited_subset 
     exact same_visited
 
   constructor
   · omega
-  · unfold bfs_step
-    split
-    · have contra : nextState.terminated = true := by 
-        clear still_not_terminated same_visited 
-        rw [nextStateDef]
-        unfold bfs_step 
-        split
-        · simp_all
-        split
-        · simp_all 
-        unfold bfs_step_expand
-        simp_all
-      simp_all
-    split -- style is bad!
-    · next _ head tail compose is_goal =>
-      have contra : nextState.terminated = true := by 
-        clear still_not_terminated same_visited 
-        rw [nextStateDef]
-        unfold bfs_step 
-        split
-        · simp_all
-        split
-        · simp_all
-        unfold bfs_step_expand
-        simp_all
-      simp_all
-    next _ head tail compose not_goal =>
-    unfold bfs_step_expand
+  · unfold bfs_step_expand
     simp_all
-    --simp [Nat.add_comm]  -- only needed for DFS not for BFS
+    simp [Nat.add_comm]
     intro a head_adj_a
-    --rw [visited_eq] -- only needed for DFS not for BFS
-    unfold bfs_step
-    split
-    · simp_all
-    split
-    · simp_all
+    rw [visited_eq]
     unfold bfs_step_expand
     simp_all
-    by_cases h : a ∈ (bfs_step g start goal priorState).1.visited
+    classical
+    by_cases h : a ∈ (bfs_step_expand g priorState head tail).visited
     · left; exact h
     · right; exact h
 
-def bfs_recurse [FinEnum V] [DecidableEq E] [DecidableEq V]
-    (g: WeightedDiGraph V E) (start : V) (goal : V)
-    (priorState : bfs_state g start)
-    (not_terminated : priorState.terminated = false):
-    (bfs_state g start) × Bool :=
-  let qq := bfs_step g start goal priorState
-  let nextState := qq.fst
-  let result := qq.snd
-  if result_is_none : result = none then 
-    let still_not_terminated : nextState.terminated = false := by
-      unfold nextState
-      unfold result at result_is_none
-      unfold qq at result_is_none ⊢
-      unfold bfs_step at result_is_none ⊢
-      split
-      · simp_all
-      · next _ head tail compose =>
-        simp_all
-        split
-        all_goals
-          simp_all -- one goal vanishes
-        unfold bfs_step_expand
-        simp_all
-    bfs_recurse g start goal nextState still_not_terminated
-  else ⟨ nextState, result.get (by apply Option.isSome_iff_ne_none.mpr ; exact result_is_none) ⟩ 
-termination_by (¬priorState.terminated, Fintype.card V - priorState.visited.card, priorState.stack.length, goal) -- must be a well-founded relation/measure
-decreasing_by
-  rw [Prod.lex_iff]
-  apply (Classical.or_iff_not_imp_left).mpr
-  simp_all
-  rw [Prod.lex_iff]
-  rw [Prod.lex_iff]
-  simp_all
-  constructor
-  · simp_all only [qq, nextState]
-  unfold nextState at still_not_terminated
-  unfold qq at still_not_terminated
-  apply termination_bfs_recurse
-  rotate_right
-  use goal
-  simp_all
-
-
-abbrev bfs_invar_over_step [FinEnum V] [DecidableEq E] [DecidableEq V]
-    (g: WeightedDiGraph V E)(start : V)(goal : V)(invar : V → bfs_state g start → Prop) :=
-      ∀ s : bfs_state g start, invar start s → invar start (bfs_step g start goal s).fst
-
-lemma bfs_recurse_lift_invar
-    (g: WeightedDiGraph V E)
-    (start : V)(priorState : bfs_state g start)
-    (not_terminated : priorState.terminated = false)
-    (invar : V → bfs_state g start → Prop):
-    ∀ (goal : V), invar start priorState ∧ (bfs_invar_over_step g start goal invar)
-     → invar start (bfs_recurse g start goal priorState not_terminated).fst := by
-      intro goal ⟨ invar_holds_initially, bfs_step_keeps_invar ⟩ 
-      unfold bfs_recurse
-      simp
-      unfold bfs_invar_over_step at bfs_step_keeps_invar
-      have h := bfs_step_keeps_invar priorState invar_holds_initially 
-
-      split
-      · next step_returns_none =>
-        have still_not_terminated : (bfs_step g start goal priorState).1.terminated = false := by
-          unfold bfs_step at ⊢ step_returns_none
-          simp_all
-          split
-          · next stack_empty =>
-            rw [stack_empty] at step_returns_none
-            simp_all
-          · simp_all
-            split
-            · next head tail compose is_goal =>
-              simp_all
-            · unfold bfs_step_expand
-              simp_all
-        exact bfs_recurse_lift_invar g start (bfs_step g start goal priorState).1 still_not_terminated invar goal ⟨ h, bfs_step_keeps_invar ⟩
-      · simp
-        exact h
-termination_by (¬priorState.terminated, Fintype.card V - priorState.visited.card, priorState.stack.length) -- must be a well-founded relation/measure
-decreasing_by
-  rw [Prod.lex_iff]
-  apply (Classical.or_iff_not_imp_left).mpr
-  simp_all
-  rw [Prod.lex_iff]
-  apply termination_bfs_recurse
-  rotate_right
-  use goal
-  simp_all
-
-lemma bfs_step_returning_non_did_not_terminate(g: WeightedDiGraph V E)
-    (start : V) (goal : V) (priorState : bfs_state g start):
-    (bfs_step g start goal priorState).2 = none → 
-    (bfs_step g start goal priorState).1.terminated = false := by
-      intro gg
-      unfold bfs_step at gg ⊢
-      split
-      · simp_all
-      · simp_all
-        split
-        · simp_all
-        · simp_all
-          unfold bfs_step_expand
-          simp_all
-
-
-lemma bfs_recurse_goal_visited_if_terminated
-    (g: WeightedDiGraph V E)
-    (start : V)(priorState : bfs_state g start)
-    (not_terminated : priorState.terminated = false)
-    (invar_stack_visited : bfs_invar_stack_is_visited g start priorState):
-    ∀ goal : V, (bfs_recurse g start goal priorState not_terminated).2 = true →
-     goal ∈ (bfs_recurse g start goal priorState not_terminated).1.visited := by
-   intro goal terminated_with_true
-   unfold bfs_recurse at terminated_with_true ⊢ 
-   simp_all
-   split
-   · simp_all
-     apply bfs_recurse_goal_visited_if_terminated
-     · apply bfs_step_keeps_stack_in_visited
-       exact invar_stack_visited
-     · exact terminated_with_true
-   · next step_did_terminate =>
-     simp_all
-     unfold bfs_step at terminated_with_true ⊢
-     split
-     · next l stack_empty =>
-       simp_all
-     · next l head tail stack_not_empty =>
-       simp_all
-       split
-       · next head_is_goal =>
-         simp_all
-       · next head_is_not_goal =>
-         simp_all
-         unfold bfs_step_expand
-         simp_all
-         by_cases goal_was_visited : goal ∈ priorState.visited
-         · left; exact goal_was_visited
-         · right
-           constructor
-           · unfold bfs_step at step_did_terminate
-             simp_all
-           · exact goal_was_visited
-termination_by (¬priorState.terminated, Fintype.card V - priorState.visited.card, priorState.stack.length) -- must be a well-founded relation/measure
-decreasing_by
-  rw [Prod.lex_iff]
-  apply (Classical.or_iff_not_imp_left).mpr
-  simp_all
-  rw [Prod.lex_iff]
-  next a b c d e f gg =>
-  clear b c d e f
-  have did_terminate_before : (bfs_step g start goal priorState).1.terminated = false := by
-    apply bfs_step_returning_non_did_not_terminate
-    exact gg
-  constructor
-  · exact did_terminate_before
-  apply termination_bfs_recurse
-  rotate_right
-  use goal
-  simp_all
-
-lemma bfs_recurse_stack_empty_if_terminated
-    (g: WeightedDiGraph V E)
-    (start : V)
-    (priorState : bfs_state g start)
-    (not_terminated : priorState.terminated = false)
-    (invar_stack_visited : bfs_invar_stack_is_visited g start priorState):
-    ∀ goal : V, (bfs_recurse g start goal priorState not_terminated).2 = false →
-     (bfs_recurse g start goal priorState not_terminated).1.stack = [] := by
-   intro goal terminated_with_false 
-   unfold bfs_recurse at terminated_with_false ⊢ 
-   simp_all
-   split
-   · next step_did_not_terminate =>
-     simp_all
-     apply bfs_recurse_stack_empty_if_terminated
-     · apply bfs_step_keeps_stack_in_visited
-       exact invar_stack_visited
-     · simp_all
-   · next step_did_terminate =>
-     simp [step_did_terminate] at terminated_with_false
-     unfold bfs_step at terminated_with_false
-     by_cases prior_stack_empty : priorState.stack = []
-     · simp [prior_stack_empty] at terminated_with_false
-       simp_all
-       unfold bfs_step
-       simp_all
-     · simp_all
-       by_cases stack_composed : ∃ a : V, ∃ l : List V, priorState.stack = a :: l
-       · obtain ⟨a,l,stack_composition⟩ := stack_composed 
-         simp_all
-         split at terminated_with_false
-         · simp_all
-         · next head_not_goal =>
-           simp_all
-           unfold bfs_step at step_did_terminate
-           simp_all
-       · have stackEmpty: priorState.stack = [] := by
-           apply List.eq_nil_of_length_eq_zero
-           unfold List.length
-           split
-           · rfl
-           · next l head tail compose=>
-             simp_all
-         simp_all
-termination_by (¬priorState.terminated, Fintype.card V - priorState.visited.card, priorState.stack.length) -- must be a well-founded relation/measure
-decreasing_by
-  rw [Prod.lex_iff]
-  apply (Classical.or_iff_not_imp_left).mpr
-  simp_all
-  rw [Prod.lex_iff]
-  next a b c d e f gg =>
-  clear b c d e f
-  have did_terminate_before : (bfs_step g start goal priorState).1.terminated = false := by
-    apply bfs_step_returning_non_did_not_terminate
-    exact gg
-  constructor
-  · exact did_terminate_before
-  apply termination_bfs_recurse
-  rotate_right
-  use goal
-  simp_all
-
-lemma bfs_recurse_if_goal_on_stack_return_true
-    (g: WeightedDiGraph V E)
-    (start : V) (priorState : bfs_state g start)
-    (not_terminated : priorState.terminated = false)
-    (invar_stack_visited : bfs_invar_stack_is_visited g start priorState):
-    ∀ goal : V, goal ∈ priorState.stack
-      → (bfs_recurse g start goal priorState not_terminated).2 = true := by
-  intro goal goal_on_stack
-  unfold bfs_recurse
-  simp
-  split
-  · apply bfs_recurse_if_goal_on_stack_return_true
-    · apply bfs_step_keeps_stack_in_visited
-      exact invar_stack_visited
-    · next step_returned_none =>
-      unfold bfs_step at step_returned_none ⊢ 
-      split
-      · next l emptyStack =>
-        simp_all
-      · next l head tail stackCompose =>
-        simp_all
-        split
-        · simp_all
-        · next head_not_goal =>
-          simp_all
-          have goal_not_head : goal ≠ head := by
-            intro a
-            apply head_not_goal
-            exact a.symm
-          simp at goal_not_head; clear head_not_goal
-          apply (Classical.or_iff_not_imp_left).mp at goal_on_stack
-          apply goal_on_stack at goal_not_head
-          unfold bfs_step_expand
-          simp_all
-  · next h =>
-    simp_all
-    unfold bfs_step
-    by_cases prior_state_non_empty: priorState.stack ≠ []
-    · simp_all
-      apply List.length_pos_iff.mpr at prior_state_non_empty
-      apply List.length_pos_iff_exists_cons.mp at prior_state_non_empty
-      obtain ⟨head,tail,compose⟩ := prior_state_non_empty
-      simp_all
-      split
-      all_goals
-        simp_all
-    · simp_all
-termination_by (¬priorState.terminated, Fintype.card V - priorState.visited.card, priorState.stack.length) -- must be a well-founded relation/measure
-decreasing_by
-  rw [Prod.lex_iff]
-  apply (Classical.or_iff_not_imp_left).mpr
-  simp_all
-  rw [Prod.lex_iff]
-  next a b c d e f gg =>
-  clear b c d e f
-  have did_terminate_before : (bfs_step g start goal priorState).1.terminated = false := by
-    apply bfs_step_returning_non_did_not_terminate
-    exact gg
-  constructor
-  · exact did_terminate_before
-  apply termination_bfs_recurse
-  rotate_right
-  use goal
-  simp_all
-
-
-lemma bfs_recurse_goal_not_visited_if_terminated
-    (g: WeightedDiGraph V E)
-    (start : V)(priorState : bfs_state g start)
-    (not_terminated : priorState.terminated = false)
-    (invar_stack_visited : bfs_invar_stack_is_visited g start priorState):
-    ∀ goal : V, (bfs_recurse g start goal priorState not_terminated).2 = false 
-    ∧ goal ∉ priorState.visited
-    → goal ∉ (bfs_recurse g start goal priorState not_terminated).1.visited := by
-  intro goal
-  intro ⟨ terminated_with_false, goal_not_visited ⟩ 
-  have new_new := terminated_with_false
-  apply bfs_recurse_stack_empty_if_terminated at terminated_with_false
-  · unfold bfs_recurse at terminated_with_false
-    simp_all
-    split at terminated_with_false
-    · next step_returns_none =>
-      unfold bfs_recurse
-      simp_all
-      apply bfs_recurse_goal_not_visited_if_terminated
-      · apply bfs_step_keeps_stack_in_visited
-        exact invar_stack_visited
-      · constructor
-        · unfold bfs_recurse at new_new
-          simp_all
-        · unfold bfs_step
-          split
-          · simp_all
-          · split
-            · simp_all
-            · next l head tail composed head_not_goal =>
-              simp_all
-              unfold bfs_step_expand
-              simp_all
-              by_contra head_adj_goal
-              have goal_is_now_on_stack : goal ∈ (bfs_step g start goal priorState).1.stack := by
-                unfold bfs_step
-                simp_all
-                unfold bfs_step_expand
-                simp_all
-              apply bfs_recurse_if_goal_on_stack_return_true at goal_is_now_on_stack
-              unfold bfs_recurse at new_new
-              simp_all
-              · unfold bfs_step
-                simp_all
-                unfold bfs_step_expand
-                simp_all
-              · apply bfs_step_keeps_stack_in_visited
-                exact invar_stack_visited
-    · unfold bfs_recurse
-      simp_all
-      unfold bfs_step at terminated_with_false ⊢
-      split
-      · simp_all
-      · simp_all
-        split
-        · simp_all
-        · simp_all
-          unfold bfs_step_expand at terminated_with_false ⊢
-          simp_all
-          next l head tail step_did_not_return_none stackCompose head_not_goal =>
-          by_contra head_adj_goal
-          have ⟨ all_adj_in_visi, tail_empty ⟩ := terminated_with_false 
-          simp_all
-  · exact invar_stack_visited
-termination_by (¬priorState.terminated, Fintype.card V - priorState.visited.card, priorState.stack.length) -- must be a well-founded relation/measure
-decreasing_by
-  rw [Prod.lex_iff]
-  apply (Classical.or_iff_not_imp_left).mpr
-  simp_all
-  rw [Prod.lex_iff]
-  next a b c d e f gg =>
-  clear b c d e f
-  have did_terminate_before : (bfs_step g start goal priorState).1.terminated = false := by
-    apply bfs_step_returning_non_did_not_terminate
-    exact gg
-  constructor
-  · exact did_terminate_before
-  apply termination_bfs_recurse
-  rotate_right
-  use goal
-  simp_all
-
-
---------------------------------------------------------------------------------------------------
--- initial configuration of the bfs
-def bfs_initial_state [FinEnum V] [DecidableEq E] [DecidableEq V]
-    (g: WeightedDiGraph V E) (start : V) (goal : V) :
-    bfs_state g start :=
-  let initialVisited : Finset V := ⟨ {start},  by simp ⟩ 
-  let initialMother : initialVisited → V := fun x => start 
-  let initialMotherProof (v : initialVisited): ↑v ≠ start → g.Adj (initialMother v) v := by
-    intro v_noit_start
-    obtain ⟨ vv, v_in_initial⟩ := v
-    simp_all
-    unfold initialVisited at v_in_initial 
-    simp at v_in_initial 
-    contradiction
-
-  let initialPathOrder : V → Nat := fun x => 0 
-  let initialStack : List V := [start]
-  bfs_state.mk initialVisited initialPathOrder initialMother initialMotherProof initialStack false
-
-
------ Proofs that the initial state of the bfs satisfies the invariants
-theorem bfs_invar_stack_is_visited_initial 
-    (g: WeightedDiGraph V E) (start : V) (goal : V) :
-      bfs_invar_stack_is_visited g start (bfs_initial_state g start goal) := by 
-      unfold bfs_invar_stack_is_visited
-      unfold bfs_initial_state
-      simp
-
-
-theorem bfs_invar_mother_is_visited_initial 
-    (g: WeightedDiGraph V E) (start : V) (goal : V) :
-      bfs_invar_mother_is_visited g start (bfs_initial_state g start goal) := by 
-      unfold bfs_invar_mother_is_visited
-      unfold bfs_initial_state
-      simp
-
-theorem bfs_invar_mother_decreasing_path_order_initial
-    (g: WeightedDiGraph V E) (start : V) (goal : V) :
-      bfs_invar_mother_decreasing_path_order g start (bfs_initial_state g start goal) := by 
-      unfold bfs_invar_mother_decreasing_path_order  
-      unfold bfs_initial_state
-      simp
-
-theorem bfs_invar_on_stack_or_all_neighbours_visited_initial
-    (g: WeightedDiGraph V E) (start : V) (goal : V) :
-      bfs_invar_on_stack_or_all_neighbours_visited g start (bfs_initial_state g start goal) := by 
-      unfold bfs_invar_on_stack_or_all_neighbours_visited  
-      unfold bfs_initial_state
-      simp
-
-theorem bfs_invar_start_visited_initial
-    (g: WeightedDiGraph V E) (start : V) (goal : V) :
-      bfs_invar_start_visited g start (bfs_initial_state g start goal) := by 
-      unfold bfs_invar_start_visited  
-      unfold bfs_initial_state
-      simp
-
-theorem bfs_initial_state_is_not_termianted (g: WeightedDiGraph V E) (start : V) (goal : V) :
-  (bfs_initial_state g start goal).terminated = false := by
-    unfold bfs_initial_state
+lemma bfs_expand_metric_reduction : termination_proof_for_expand (g:=g) goal (bfs_step_expand g) base_search_state_termination_metric := by
+    unfold termination_proof_for_expand
+    unfold base_search_state_termination_metric
     simp
-
+    intro s head tail head_not_goal stack_not_empty 
+    apply termination_bfs_recurse
+    · exact stack_not_empty
+    · rfl 
 
 
 ----------------- the actual bfs: create the initial search state and then recurse
 
-def bfs_internal[ FinEnum V] [DecidableEq E] [DecidableEq V]
-    (g: WeightedDiGraph V E) (start : V) (goal : V): (bfs_state g start) × Bool :=
-  (bfs_recurse g start goal (bfs_initial_state g start goal) (bfs_initial_state_is_not_termianted g start goal))
+def bfs(g: WeightedDiGraph V E) (start : V) (goal : V): Option (Path g start goal) :=
+  let start_state := base_search_state_initial start
+  have h : has_base_search_state.to_base_state (g:=g) start_state = base_search_state_initial start:= by simp_all only [start_state]; rfl
 
+  search_exe_with_stack_step (g:=g) (start := start) (goal:=goal) (start_state:=start_state) (termination_metric := base_search_state_termination_metric) (bfs_step_expand g) bfs_expand_metric_reduction bfs_expand_keeps_base_invars h 
 
-
-lemma bfs_returns_correct_results 
-    (g: WeightedDiGraph V E) (start : V) (goal : V) (final : bfs_state g start):
-    final = (bfs_internal g start goal).1 →
-      bfs_invar_start_visited g start final
-    ∧ bfs_invar_on_stack_or_all_neighbours_visited g start final
-    ∧ bfs_invar_stack_is_visited g start final
-    ∧ bfs_invar_mother_is_visited g start final
-    ∧ bfs_invar_mother_decreasing_path_order g start final
-    ∧ ((bfs_internal g start goal).2 = true → goal ∈ final.visited)
-    ∧ ((bfs_internal g start goal).2 = false → goal ∉ final.visited ∧ final.stack = []) := by
-    
-    intro s_is_final
-
-    let startState : bfs_state g start := bfs_initial_state g start goal
-    let proof : startState.terminated = false := bfs_initial_state_is_not_termianted g start goal
-    rw [s_is_final]
-    clear s_is_final final
-    let final := (bfs_internal g start goal).1
-
-    rw [← and_assoc]
-    rw [← and_assoc]
-    rw [← and_assoc]
-    rw [← and_assoc]
-    
-    have five_invars :
-          bfs_invar_start_visited g start final
-        ∧ bfs_invar_on_stack_or_all_neighbours_visited g start final
-        ∧ bfs_invar_stack_is_visited g start final
-        ∧ bfs_invar_mother_is_visited g start final
-        ∧ bfs_invar_mother_decreasing_path_order g start final := by
-      apply bfs_recurse_lift_invar g start startState proof (fun st s =>
-          bfs_invar_start_visited g start s 
-        ∧ bfs_invar_on_stack_or_all_neighbours_visited g start s
-        ∧ bfs_invar_stack_is_visited g start s
-        ∧ bfs_invar_mother_is_visited g start s
-        ∧ bfs_invar_mother_decreasing_path_order g start s) goal
-      constructor
-      · rw [← and_assoc]
-        rw [← and_assoc]
-        rw [← and_assoc]
-        repeat constructor
-        · apply bfs_invar_on_stack_or_all_neighbours_visited_initial
-        · apply bfs_invar_stack_is_visited_initial
-        · apply bfs_invar_mother_is_visited_initial
-        · apply bfs_invar_mother_decreasing_path_order_initial
-      unfold bfs_invar_over_step
-      intro s
-      intro ⟨ start_visited, nei_visited, stack_visited, mother_visited, mother_decreasing⟩
-      rw [← and_assoc]
-      rw [← and_assoc]
-      rw [← and_assoc]
-      repeat constructor
-      · apply bfs_step_keeps_start_in_visited
-        exact start_visited
-      · apply bfs_step_keeps_on_stack_or_all_neighbours_visited 
-        exact nei_visited
-      · apply bfs_step_keeps_stack_in_visited
-        exact stack_visited
-      · apply bfs_step_keeps_mother_in_visited
-        exact ⟨ stack_visited, mother_visited ⟩ 
-      · apply bfs_step_keeps_mother_ordered
-        exact ⟨ stack_visited, mother_visited, mother_decreasing⟩ 
-
-    constructor
-    · apply and_assoc.mpr
-      apply and_assoc.mpr
-      apply and_assoc.mpr
-      exact five_invars
-    -- prove the the properties for the two termination cases
-    constructor
-    · intro terminated_with_goal_found
-      apply bfs_recurse_goal_visited_if_terminated
-      apply bfs_invar_stack_is_visited_initial
-      unfold bfs_internal at terminated_with_goal_found
-      exact terminated_with_goal_found
-    · intro terminated_with_goal_not_found
-      repeat constructor
-      · apply bfs_recurse_goal_not_visited_if_terminated
-        apply bfs_invar_stack_is_visited_initial
-        constructor
-        · unfold bfs_internal at terminated_with_goal_not_found
-          simp_all
-        · unfold bfs_initial_state
-          simp_all
-          by_contra goal_is_start
-          unfold bfs_internal at terminated_with_goal_not_found
-          simp_all
-          unfold bfs_recurse at terminated_with_goal_not_found
-          simp_all
-          unfold bfs_initial_state at terminated_with_goal_not_found
-          unfold bfs_step at terminated_with_goal_not_found
-          simp_all
-      · apply bfs_recurse_stack_empty_if_terminated
-        apply bfs_invar_stack_is_visited_initial
-        unfold bfs_internal at terminated_with_goal_not_found
-        exact terminated_with_goal_not_found
-
-def bfs [FinEnum V] [DecidableEq E] [DecidableEq V]
-    (g: WeightedDiGraph V E) (start : V) (goal : V): Option (Path g start goal) :=
-
-  let bfs_ret := bfs_internal g start goal
-  let final_state :=bfs_ret.1
-  let found_goal := bfs_ret.2
-
-  if found_goal_true : found_goal = true then
-    have xx := bfs_returns_correct_results g start goal final_state (by
-      unfold final_state 
-      unfold bfs_ret
-      rfl)
-    some (extract_path_to g start goal final_state (xx.2.2.2.2.2.1 found_goal_true) xx.2.2.2.1 xx.2.2.2.2.1).1
-  else
-    none
 
 
 theorem bfs_is_sound (g: WeightedDiGraph V E) (start : V) (goal : V) :
     (Option.isSome (bfs g start goal) → (∃ x : (Path g start goal), x = x)) := by
-  intro h -- Option.isSome true on some and false on none, x = x since we need a formula
-  constructor -- since goal is existence
-  rfl
-  let w := Option.get (bfs g start goal) -- Option.get extracts value of returned some and fails otherwise
-  apply w
-  simp_all
+  apply search_with_stack_step_is_sound
+  · apply bfs_expand_metric_reduction
+  · apply bfs_expand_keeps_base_invars
+  · rfl
 
 
-lemma my_induction (g: WeightedDiGraph V E) (start : V) (goal : V) (f : V) 
-  (theWalk : Walk g f goal)
-  (final_state : bfs_state g start)
-  (f_visited : f ∈ final_state.visited)
-  (final_stack_empty : final_state.stack = [])
-  (on_stack_or_all_nei_visited : ∀ a ∈ final_state.visited, ∀ (y : V), g.Adj a y → y ∈ final_state.visited): goal ∈ final_state.visited := by
-    cases theWalk
-    · exact f_visited
-    · next nextNode adj rest_walk =>
-      apply my_induction g start goal nextNode rest_walk
-      · apply on_stack_or_all_nei_visited f
-        · exact f_visited
-        · exact adj
-      · exact final_stack_empty
-      · exact on_stack_or_all_nei_visited
 
-
-theorem bfs_is_complete (g: WeightedDiGraph V E) (start : V) (goal : V) :
+theorem bfs_is_complete (g: WeightedDiGraph V E) (start : V) (goal : V):
     ((∃ x : (Path g start goal), x = x) → Option.isSome (bfs g start goal)) := by
-    -- or Option.isNone (bfs g start goal) → ∄ x (Path g start goal), x = x
-      intro path_exists
-      apply Exists.elim path_exists
-      intro thePath
-      intro a; clear a-- uninformativ x=X
-      
-      by_contra terminates_with_none
-      simp at terminates_with_none
-
-      let final := bfs_internal g start goal
-      let final_state := final.1
-
-      have xx := bfs_returns_correct_results g start goal final_state (by
-        unfold final_state 
-        unfold final
-        rfl)
-
-      have h := xx.2.2.2.2.2.2
-      have start_visited := xx.1
-      unfold bfs_invar_start_visited at start_visited
-      have on_stack_or_all_nei_visited := xx.2.1
-      clear xx
-      unfold bfs at terminates_with_none
-      simp at terminates_with_none
-      apply h at terminates_with_none
-      clear h
-      simp_all
-      obtain ⟨goal_not_visited, final_stack_empty⟩ := terminates_with_none
-
-      obtain ⟨theWalk, nodupe ⟩ := thePath
-      have goal_in_final := my_induction g start goal start theWalk final_state start_visited final_stack_empty on_stack_or_all_nei_visited
-      contradiction
-
-
-theorem bfs_is_complete_inv (g: WeightedDiGraph V E) (start : V) (goal : V) :
-    Option.isNone (bfs g start goal) → ¬ ∃ x : (Path g start goal), x = x := by
-      intro optionIsNone
-      by_contra pathExists
-      have isSome := bfs_is_complete g start goal pathExists
-      simp_all
+  apply search_with_stack_step_is_complete
+  · apply bfs_expand_metric_reduction
+  · apply bfs_expand_keeps_base_invars
+  · rfl
+  · apply bfs_expand_keeps_goal_on_stack
+  · apply bfs_expand_goal_becomes_visited_puts_it_on_stack
 
